coqimp/framework/soundness/wf_seq_sound.v
@@ -1,4 +1,4 @@
-Require Import Coqlib.       
+Require Import Coqlib.        
 Require Import Maps.      
 Require Import LibTactics.  
        
@@ -130,17 +130,16 @@ Qed.
     
 (*+ Lemmas for Safety Instruction Sequence +*)
 Lemma safety_ins_seq_post_weak :
-  forall I C S pc npc q q' Spec,
-    LookupC C pc npc I ->
-    safety_insSeq C S pc npc q Spec -> q ==> q' ->
-    safety_insSeq C S pc npc q' Spec.
+  forall I C S pc q q' Spec,
+    LookupC C pc I ->
+    safety_insSeq C S pc (pc +ᵢ ($ 4)) q Spec -> q ==> q' ->
+    safety_insSeq C S pc (pc +ᵢ ($ 4)) q' Spec.
 Proof.
   intro I.
   induction I; intros.
   
   - (** i *)
     inversion H; subst.
-    renames l to pc.
     inversion H0; get_ins_diff_false.
     eapply i_seq; eauto.
     intros.
@@ -149,38 +148,24 @@ Proof.
     clear H2 H H3.
     inversion H5; subst.
     inversion H13; get_ins_diff_false; subst.
-    clear - IHI H9 Hsafety H1.
+    clear - IHI H7 Hsafety H1.
     eauto.
 
   - (** J1 *)
     inversion H; subst.
-    renames l to pc, l0 to npc.
     inversion H0; get_ins_diff_false.
     eapply jmpl_seq; eauto.
     intros.
     clear H3 H2.
-    lets Hp : H6.
+    lets Hp : H7.
     eapply H4 in Hp; eauto.
     simpljoin1.
     renames x to fp, x1 to L, x0 to fq, x2 to r.
     exists fp fq L r.
     repeat (split; eauto).
 
-  - (** J2 *)
-    inversion H; subst.
-    renames l to pc, l0 to npc.
-    inversion H0; get_ins_diff_false.
-    eapply jmpl_seq; eauto.
-    intros.
-    eapply H4 in H6; eauto.
-    simpljoin1.
-    renames x to fp, x0 to fq, x1 to L, x2 to r.
-    exists fp fq L r.
-    repeat (split; eauto).
-
   - (** call f *)
     inversion H; subst.
-    renames l to pc.
     inversion H0; get_ins_diff_false.
     eapply call_seq; eauto.
     clear H2 H3.
@@ -191,26 +176,26 @@ Proof.
     exists fp fq L r.
     repeat (split; eauto).
     intros.
-    eapply H10 in H3.
+    eapply H12 in H3.
+    assert (pc +ᵢ ($ 12) = (pc +ᵢ ($ 8)) +ᵢ ($ 4)).
+    rewrite Int.add_assoc; eauto.
+    rewrite H5.
     eapply IHI; eauto.
-    clear - H13.
-    do 2 rewrite Int.add_assoc in H13.
-    simpls; eauto.
+    rewrite <- H5.
+    eauto.
 
   - (** retl *)
     inversion H; subst.
-    renames l to pc, l0 to npc.
     inversion H0; get_ins_diff_false.
     eapply ret_seq; eauto.
-    clear H2 H3.
+    clear H2 H4.
     intros.
-    eapply H4 in H3; eauto.
+    eapply H5 in H4; eauto.
     simpljoin1; eauto.
     split; eauto.
 
   - (** be *) 
     inversion H; subst.
-    renames l to pc, l0 to npc.
     inversion H0; get_ins_diff_false.
     eapply be_seq; eauto.
     clear H2 H3.
@@ -221,12 +206,12 @@ Proof.
     exists x.
     repeat (split; eauto).
     intros.
-    eapply H5 in H7.
+    eapply H5 in H10.
     simpljoin1.
     do 4 eexists.
     repeat (split; eauto).
     intros.
-    lets Hfalse : H7.
+    lets Hfalse : H10.
     eapply H6 in Hfalse.
     inversion H2; subst.
     inversion H19; get_ins_diff_false.
@@ -242,13 +227,12 @@ Proof.
     inversion Hp; subst.
     inversion H24; get_ins_diff_false.
     eapply IHI; eauto. 
-    clear - H12.
+    clear - H9.
     rewrite Int.add_assoc.
     eauto.
 
   - (** bne *)
     inversion H; subst.
-    renames l to pc, l0 to npc.
     inversion H0; get_ins_diff_false.
     eapply bne_seq; eauto.
     clear H2 H3.
@@ -259,14 +243,14 @@ Proof.
     exists x.
     repeat (split; eauto).
     intros.
-    eapply H5 in H7.
+    eapply H5 in H10.
     simpljoin1.
     renames x0 to fp, x1 to fq, x2 to L, x3 to r.
     exists fp fq L r.
     repeat (split; eauto).
     intros.
-    lets Hfalse : H7.
-    eapply H6 in H7.
+    lets Hfalse : H10.
+    eapply H6 in H10.
     inversion H2; subst.
     inversion H19; get_ins_diff_false.
     simpl in H3. 
@@ -281,23 +265,23 @@ Proof.
     inversion Hp; subst.
     inversion H25; get_ins_diff_false.
     eapply IHI; eauto.
-    clear - H12.
+    clear - H9.
     rewrite Int.add_assoc.
     eauto.
 Qed.
 
 Lemma safety_ins_seq_frame_property :
-  forall I C pc npc q r Spec m0 m1 r0 r1 f0 d0,
-    LookupC C pc npc I -> (m0, (r0, f0), d0) |= r -> DlyFrameFree r ->
-    disjoint m1 m0 -> disjoint r1 r0 -> safety_insSeq C (m1, (r1, f0), d0) pc npc q Spec ->
-    safety_insSeq C (merge m1 m0, (merge r1 r0, f0), d0) pc npc (q ** r) Spec.
+  forall I C pc q r Spec m0 m1 r0 r1 f0 d0,
+    LookupC C pc I -> (m0, (r0, f0), d0) |= r -> DlyFrameFree r ->
+    disjoint m1 m0 -> disjoint r1 r0 ->
+    safety_insSeq C (m1, (r1, f0), d0) pc (pc +ᵢ ($ 4)) q Spec ->
+    safety_insSeq C (merge m1 m0, (merge r1 r0, f0), d0) pc (pc +ᵢ ($ 4)) (q ** r) Spec.
 Proof.
   intro I.
   induction I; intros.
 
   - (** i *)
     inversion H; subst.
-    renames l to pc.
     inversion H4; get_ins_diff_false.
     eapply i_seq; eauto.
     {
@@ -309,7 +293,7 @@ Proof.
       eauto.
       simpl; eauto.
     }
-    {
+    { 
       simpljoin1.
       lets Hsafety : H6.
       eapply H7 in Hsafety.
@@ -324,16 +308,15 @@ Proof.
       intros.
       eapply program_step_deterministic in H5; eauto.
       simpljoin1.
-      eapply IHI; eauto.
-      inversion H9; subst.
+      lets Hsetp : H11.
+      inversion H11; subst.
       inversion H25; get_ins_diff_false.
-      eauto.
+      eapply IHI; eauto.
       simpl; eauto.
     }
 
   - (** J1 *)
     inversion H; subst.
-    renames l to pc, l0 to npc.
     inversion H4; get_ins_diff_false.
     eapply jmpl_seq; eauto. 
     simpljoin1.
@@ -363,90 +346,26 @@ Proof.
         eauto.
       simpljoin1.
       destruct_state x.
-      destruct_state x6.
+      destruct_state x5.
       simpl in H16.
-      simpljoin1.
+      simpljoin1. 
       eapply program_step_safety_property with
-      (s := (m ⊎ m2, (r2 ⊎ r3, f1), d1)) (r := r) in H11;
+      (s := (m ⊎ m2, (r2 ⊎ r3, f1), d1)) (r := r) in H12;
         eauto.
       simpljoin1.
       destruct_state x0.
-      destruct_state x5.
+      destruct_state x4.
       simpl in H19.
       simpljoin1.
       clear H7.
       eapply program_step_deterministic in H6; eauto.
       simpljoin1.
-      eapply program_step_deterministic in H11; eauto.
-      simpljoin1.
-      exists fp fq L (r' ** r).
-      eapply disj_sep_star_merge with (p2 := r) in H12; eauto.
-      eapply sep_star_assoc2 in H12.
-      repeat (split; eauto).
-      intros.
-      eapply sep_star_assoc in H6.
-      eapply sep_star_subst; eauto.
-      simpl; eauto.
-      simpl; eauto.
-    }
-
-  - (** J2 *)
-    inversion H; subst.
-    renames l to pc, l0 to npc.
-    inversion H4; get_ins_diff_false.
-    eapply jmpl_seq; eauto.
-    simpljoin1.
-    {
-      clear H7.
-      eapply program_step_safety_property with (s := (m1 ⊎ m0, (r1 ⊎ r0, f0), d0)) in H6;
-        eauto.
-      simpljoin1.
-      destruct_state x.
-      destruct_state x6.
-      simpls.
-      simpljoin1.
-      eapply program_step_safety_property with (s := (m ⊎ m2, (r2 ⊎ r3, f1), d1)) in H8;
-        eauto.
-      simpljoin1.
-      destruct_state x0.
-      destruct_state x5.
-      simpls.
-      simpljoin1.
-      do 6 eexists.
-      eauto.
-      simpl; eauto.
-      simpl; eauto.
-    }
-    {
-      simpljoin1.
-      lets Hp : H6. 
-      eapply H7 with (S1 := x) in Hp; eauto.
-      simpljoin1.
-      renames x5 to fp, x6 to fq, x7 to L, x8 to r'.
-      clear H7. 
-      eapply program_step_safety_property with (s := (m1 ⊎ m0, (r1 ⊎ r0, f0), d0)) (r := r)
-        in H6; eauto.
-      simpljoin1.
-      destruct_state x.
-      destruct_state x6.
-      simpl in H7.
+      eapply program_step_deterministic in H12; eauto.
       simpljoin1. 
-      eapply program_step_safety_property with (s := (m ⊎ m2, (r2 ⊎ r3, f1), d1)) (r := r)
-        in H8; eauto.
-      simpljoin1.
-      destruct_state x0.
-      destruct_state x5.
-      simpl in H16.
-      simpljoin1.
-      intros.
-      eapply program_step_deterministic in H6; eauto.
-      simpljoin1.
-      eapply program_step_deterministic in H8; eauto.
-      simpljoin1.
-      exists fp fq L (r' ** r).
+      exists fp fq L (r' ** r). 
+      eapply disj_sep_star_merge with (p2 := r) in H13; eauto.
+      eapply sep_star_assoc2 in H13.
       repeat (split; eauto).
-      eapply disj_sep_star_merge with (p2 := r) in H9; eauto.
-      eapply sep_star_assoc2 in H9; eauto.
       intros.
       eapply sep_star_assoc in H6.
       eapply sep_star_subst; eauto.
@@ -456,7 +375,6 @@ Proof.
 
   - (** call f *)
     inversion H; subst.
-    renames l to pc.
     inversion H4; get_ins_diff_false.
     eapply call_seq; eauto.
     {
@@ -509,7 +427,7 @@ Proof.
       simpljoin1.
       exists fp fq L (r' ** r).
       repeat (split; eauto).
-      eapply disj_sep_star_merge with (p2 := r) in H10; eauto.
+      eapply disj_sep_star_merge with (p2 := r) in H13; eauto.
       eapply sep_star_assoc2; eauto.
       intros.
       eapply sep_star_assoc in H5.
@@ -519,10 +437,12 @@ Proof.
       destruct_state x0.
       simpl in H23.
       simpljoin1.
-      eapply H13 in H5.
-      eapply IHI; eauto.
-      clear - H16.
-      do 2 rewrite Int.add_assoc in H16.
+      assert (pc +ᵢ ($ 12) = (pc +ᵢ ($ 8)) +ᵢ ($ 4)).
+      rewrite Int.add_assoc; eauto.
+      rewrite H25. 
+      eapply H15 in H5.
+      eapply IHI; eauto. 
+      rewrite <- H25.
       eauto.
       simpl; eauto.
       simpl; eauto.
@@ -530,7 +450,6 @@ Proof.
 
   - (** retl *)
     inversion H; subst.
-    renames l to pc, l0 to npc.
     inversion H4; subst; get_ins_diff_false.
     clear H H5.
     eapply ret_seq; eauto.
@@ -541,14 +460,14 @@ Proof.
       simpljoin1.
       destruct_state x.
       destruct_state x6.
-      simpl in H6.
+      simpl in H7.
       simpljoin1.
       eapply program_step_safety_property with (s := (m ⊎ m2, (r2 ⊎ r3, f1), d1))
         in H5; eauto.
       simpljoin1.
       destruct_state x0.
       destruct_state x5.
-      simpl in H11.
+      simpl in H12.
       simpljoin1.
       do 6 eexists.
       eauto.
@@ -558,15 +477,15 @@ Proof.
     {
       simpljoin1.
       lets Hp : H.
-      eapply H7 with (S1 := x) in Hp; eauto.
+      eapply H8 with (S1 := x) in Hp; eauto.
       simpljoin1.
-      clear H7.
+      clear H8.
       eapply program_step_safety_property with
       (s := (m1 ⊎ m0, (r1 ⊎ r0, f0), d0)) (r := r) in H; eauto.
       simpljoin1.
       destruct_state x.
       destruct_state x4.
-      simpl in H7.
+      simpl in H8.
       simpljoin1.
       eapply program_step_safety_property with
       (s := (m ⊎ m2, (r2 ⊎ r3, f1), d1)) (r := r) in H5; eauto.
@@ -595,7 +514,6 @@ Proof.
 
   - (** be f *)
     inversion H; subst.
-    renames l to pc, l0 to npc.
     inversion H4; subst; get_ins_diff_false.
     clear H H5.
     eapply be_seq; eauto.
@@ -636,7 +554,7 @@ Proof.
       simpljoin1.
       destruct_state x0.
       destruct_state x6.
-      simpl in H13.
+      simpl in H15.
       simpljoin1.
       intros.
       eapply program_step_deterministic in H8; eauto.
@@ -664,23 +582,22 @@ Proof.
       {
         intros.
         lets Hfalse : H5.
-        eapply H7 in H5.
-        eapply IHI; eauto.
+        eapply H7 in H5. 
         inversion H18; subst.   
         inversion H33; get_ins_diff_false.
         rewrite get_R_rn_neq_r0 in H; eauto.
         rewrite get_R_rn_neq_r0 in H35; eauto.
         eapply regz_exe_delay_stable2 in H35; eauto.
-        clear - H H35 H36. 
-        unfold merge in *.
-        rewrite H in H35; eauto.
-        inversion H35; subst.
+        eapply get_vl_merge_still in H; eauto.
+        rewrite H35 in H.
+        inversion H; subst.
         tryfalse.
         intro; tryfalse.
         intro; tryfalse.
         inversion H19; subst. 
         inversion H38; get_ins_diff_false.
-        clear - H15.
+        eapply IHI; eauto.
+        clear - H12.
         rewrite Int.add_assoc; eauto.
       }
 
@@ -690,7 +607,6 @@ Proof.
 
   - (** bne aexp *)
     inversion H; subst.
-    renames l to pc, l0 to npc.
     inversion H4; subst; get_ins_diff_false.
     clear H H5.
     eapply bne_seq; eauto.
@@ -730,7 +646,7 @@ Proof.
       simpljoin1.
       destruct_state x0.
       destruct_state x5.
-      simpl in H13.
+      simpl in H15.
       simpljoin1.
       intros.
       eapply program_step_deterministic in H; eauto.
@@ -755,22 +671,23 @@ Proof.
 
       intros.
       lets Hfalse : H.
-      eapply H10 in H.
-      eapply IHI; eauto.
+      eapply H13 in H.
       inversion H18; subst. 
       inversion H33; get_ins_diff_false; subst.
       rewrite get_R_rn_neq_r0 in H6; eauto. 
       rewrite get_R_rn_neq_r0 in H35; eauto.
-      eapply regz_exe_delay_stable2 in H35; eauto. 
-      unfold merge in H35. 
-      rewrite H6 in H35. 
+      eapply regz_exe_delay_stable2 in H35; eauto.
+      eapply get_vl_merge_still in H6; eauto.
+      rewrite H6 in H35.
       inversion H35; subst.
       tryfalse.
       intro; tryfalse.
       intro; tryfalse.
+
       inversion H19; subst.
       inversion H39; get_ins_diff_false.
-      clear - H15.
+      eapply IHI; eauto.
+      clear - H12.
       rewrite Int.add_assoc; eauto.
 
       simpl; eauto.
@@ -779,17 +696,16 @@ Proof.
 Qed.
 
 Lemma safety_ins_seq_post_disj1 :
-  forall I q1 q2 pc npc Spec C S,
-    LookupC C pc npc I ->
-    safety_insSeq C S pc npc q1 Spec ->
-    safety_insSeq C S pc npc (q1 \\// q2) Spec.
+  forall I q1 q2 pc Spec C S,
+    LookupC C pc I ->
+    safety_insSeq C S pc (pc +ᵢ ($ 4)) q1 Spec ->
+    safety_insSeq C S pc (pc +ᵢ ($ 4)) (q1 \\// q2) Spec.
 Proof.
   intro I.
   induction I; intros.
 
   - (** i *)
     inversion H; subst.
-    renames l to pc.
     inversion H0; get_ins_diff_false.
     clear H1.
     eapply i_seq; eauto.
@@ -802,7 +718,6 @@ Proof.
 
   - (** J1 *)
     inversion H; subst.
-    renames l to pc, l0 to npc.
     inversion H0; get_ins_diff_false.
     eapply jmpl_seq; eauto.
     intros.
@@ -813,28 +728,10 @@ Proof.
     exists fp fq L r.
     repeat (split; eauto).
     intros.
-    eapply H9 in H1; simpl; eauto.
-
-  - (** J2 *)
-    inversion H; subst.
-    renames l to pc, l0 to npc.
-    inversion H0; get_ins_diff_false.
-    clear H1.
-    eapply jmpl_seq; eauto.
-    intros.
-    lets Hq1 : H1.
-    eapply H3 with (S1 := S1) in Hq1; eauto.
-    simpljoin1.
-    renames x to fp, x0 to fq, x1 to L, x2 to r.
-    exists fp fq L r.
-    repeat (split; eauto).
-    intros.
-    eapply H8 in H12; eauto.
-    simpl; eauto.
+    eapply H10 in H1; simpl; eauto.
 
   - (** call *)
     inversion H; subst.
-    renames l to pc.
     inversion H0; get_ins_diff_false.
     eapply call_seq; eauto.
     intros.
@@ -845,25 +742,28 @@ Proof.
     exists fp fq L r.
     repeat (split; eauto).
     intros.
+    assert (pc +ᵢ ($ 12) = (pc +ᵢ ($ 8)) +ᵢ ($ 4)).
+    {
+      rewrite Int.add_assoc; eauto.
+    }
+    rewrite H9.
     eapply H14 in H1; eauto.
     eapply IHI; eauto.
-    clear - H12.
-    do 2 rewrite Int.add_assoc in H12; eauto.
+    rewrite <- H9.
+    eauto.
 
   - (** retl *)
     inversion H; subst.
-    renames l to pc, l0 to npc.
     inversion H0; get_ins_diff_false.
     eapply ret_seq; eauto.
     intros.
-    lets Hq1 : H4.
-    eapply H3 with (S1 := S1) in Hq1; eauto.
+    lets Hq1 : H6.
+    eapply H4 with (S1 := S1) in Hq1; eauto.
     simpljoin1.
     split; simpl; eauto.
 
   - (** be *)
     inversion H; subst.
-    renames l to pc, l0 to npc.
     inversion H0; get_ins_diff_false.
     eapply be_seq; eauto.
     intros.
@@ -873,7 +773,7 @@ Proof.
     exists x.
     repeat (split; eauto).
     intro.
-    eapply H8 in H1.
+    eapply H10 in H1.
     simpljoin1.
     exists x6 x7 x8 x9.
     repeat (split; eauto).
@@ -881,27 +781,26 @@ Proof.
     simpl; eauto.
     intro.
     lets Hx : H1.
-    eapply H9 in H1.
-    eapply IHI; eauto.
+    eapply H11 in H1.
     inversion H4; subst. 
     inversion H21; get_ins_diff_false.
-    simpl in H6.
-    rewrite get_R_rn_neq_r0 in H6; eauto.
+    simpl in H9.
+    rewrite get_R_rn_neq_r0 in H9; eauto.
     rewrite get_R_rn_neq_r0 in H29; eauto.
     eapply regz_exe_delay_stable2 in H29; eauto.
-    rewrite H6 in H29.
+    rewrite H9 in H29.
     inversion H29; subst.
     tryfalse.
     intro; tryfalse.
     intro; tryfalse.
     inversion H5; subst.
     inversion H27; get_ins_diff_false.
-    clear - H11.
+    eapply IHI; eauto.
+    clear - H8.
     rewrite Int.add_assoc; eauto.
 
   - (** bne *)
     inversion H; subst.
-    renames l to pc, l0 to npc.
     inversion H0; get_ins_diff_false.
     eapply bne_seq; eauto.
     intros.
@@ -912,44 +811,43 @@ Proof.
     repeat (split; eauto).
     intros.
     lets Hx : H1.
-    eapply H8 in H1; eauto.
+    eapply H10 in H1; eauto.
     simpljoin1.
     exists x6 x7 x8 x9.
     repeat (split; eauto).
     intros; simpl; eauto.
     intros.
-    lets Hx : H1.
-    eapply H9 in H1; eauto.
-    eapply IHI; eauto.
+    lets Hx : H1. 
+    eapply H11 in H1; eauto.
     inversion H4; subst.
     inversion H21; get_ins_diff_false.
-    simpl in H6.
-    rewrite get_R_rn_neq_r0 in H6; eauto.
+    simpl in H9.
+    rewrite get_R_rn_neq_r0 in H9; eauto.
     rewrite get_R_rn_neq_r0 in H29; eauto.
     eapply regz_exe_delay_stable2 in H29; eauto.
-    rewrite H6 in H29.
+    rewrite H9 in H29.
     inversion H29; subst.
     tryfalse.
     intro; tryfalse.
     intro; tryfalse.
     inversion H5; subst.
     inversion H27; get_ins_diff_false.
-    clear - H11.
+    eapply IHI; eauto.
+    clear - H8.
     rewrite Int.add_assoc; eauto.
 Qed.
 
 Lemma safety_ins_seq_post_disj2 :
-  forall I q1 q2 pc npc Spec C S,
-    LookupC C pc npc I ->
-    safety_insSeq C S pc npc q2 Spec ->
-    safety_insSeq C S pc npc (q1 \\// q2) Spec.
+  forall I q1 q2 pc Spec C S,
+    LookupC C pc I ->
+    safety_insSeq C S pc (pc +ᵢ ($ 4)) q2 Spec ->
+    safety_insSeq C S pc (pc +ᵢ ($ 4)) (q1 \\// q2) Spec.
 Proof.
   intro I.
   induction I; intros.
 
   - (** i *)
     inversion H; subst.
-    renames l to pc.
     inversion H0; get_ins_diff_false.
     clear H1.
     eapply i_seq; eauto.
@@ -962,7 +860,6 @@ Proof.
 
   - (** J1 *)
     inversion H; subst.
-    renames l to pc, l0 to npc.
     inversion H0; get_ins_diff_false.
     eapply jmpl_seq; eauto.
     intros.
@@ -973,28 +870,10 @@ Proof.
     exists fp fq L r.
     repeat (split; eauto).
     intros.
-    eapply H9 in H1; simpl; eauto.
-
-  - (** J2 *)
-    inversion H; subst.
-    renames l to pc, l0 to npc.
-    inversion H0; get_ins_diff_false.
-    clear H1.
-    eapply jmpl_seq; eauto.
-    intros.
-    lets Hq1 : H1.
-    eapply H3 with (S1 := S1) in Hq1; eauto.
-    simpljoin1.
-    renames x to fp, x0 to fq, x1 to L, x2 to r.
-    exists fp fq L r.
-    repeat (split; eauto).
-    intros.
-    eapply H8 in H12; eauto.
-    simpl; eauto.
+    eapply H10 in H1; simpl; eauto.
 
   - (** call *)
     inversion H; subst.
-    renames l to pc.
     inversion H0; get_ins_diff_false.
     eapply call_seq; eauto.
     intros.
@@ -1006,24 +885,25 @@ Proof.
     repeat (split; eauto).
     intros.
     eapply H14 in H1; eauto.
+    assert (pc +ᵢ ($ 12) = (pc +ᵢ ($ 8)) +ᵢ ($ 4)).
+    rewrite Int.add_assoc; eauto.
+    rewrite H9.
     eapply IHI; eauto.
-    clear - H12.
-    do 2 rewrite Int.add_assoc in H12; eauto.
+    rewrite <- H9.
+    eauto.
 
   - (** retl *)
     inversion H; subst.
-    renames l to pc, l0 to npc.
     inversion H0; get_ins_diff_false.
     eapply ret_seq; eauto.
     intros.
-    lets Hq1 : H4.
-    eapply H3 with (S1 := S1) in Hq1; eauto.
+    lets Hq1 : H6.
+    eapply H4 with (S1 := S1) in Hq1; eauto.
     simpljoin1.
     split; simpl; eauto.
 
   - (** be *)
     inversion H; subst.
-    renames l to pc, l0 to npc.
     inversion H0; get_ins_diff_false.
     eapply be_seq; eauto.
     intros.
@@ -1033,7 +913,7 @@ Proof.
     exists x.
     repeat (split; eauto).
     intro.
-    eapply H8 in H1.
+    eapply H10 in H1.
     simpljoin1.
     exists x6 x7 x8 x9.
     repeat (split; eauto).
@@ -1041,27 +921,26 @@ Proof.
     simpl; eauto.
     intro.
     lets Hx : H1.
-    eapply H9 in H1.
-    eapply IHI; eauto.
+    eapply H11 in H1.
     inversion H4; subst.
     inversion H21; get_ins_diff_false.
-    simpl in H6.
-    rewrite get_R_rn_neq_r0 in H6; eauto.
+    simpl in H9.
+    rewrite get_R_rn_neq_r0 in H9; eauto.
     rewrite get_R_rn_neq_r0 in H29; eauto.
     eapply regz_exe_delay_stable2 in H29; eauto.
-    rewrite H6 in H29.
+    rewrite H9 in H29.
     inversion H29; subst.
     tryfalse.
     intro; tryfalse.
     intro; tryfalse.
     inversion H5; subst.
     inversion H27; get_ins_diff_false.
-    clear - H11.
+    eapply IHI; eauto.
+    clear - H8.
     rewrite Int.add_assoc; eauto.
 
   - (** bne *)
     inversion H; subst.
-    renames l to pc, l0 to npc.
     inversion H0; get_ins_diff_false.
     eapply bne_seq; eauto.
     intros.
@@ -1072,37 +951,37 @@ Proof.
     repeat (split; eauto).
     intros.
     lets Hx : H1.
-    eapply H8 in H1; eauto.
+    eapply H10 in H1; eauto.
     simpljoin1.
     exists x6 x7 x8 x9.
     repeat (split; eauto).
     intros; simpl; eauto.
     intros.
     lets Hx : H1.
-    eapply H9 in H1; eauto.
-    eapply IHI; eauto.
+    eapply H11 in H1; eauto.
     inversion H4; subst.
     inversion H21; get_ins_diff_false.
-    simpl in H6.
-    rewrite get_R_rn_neq_r0 in H6; eauto.
+    simpl in H9.
+    rewrite get_R_rn_neq_r0 in H9; eauto.
     rewrite get_R_rn_neq_r0 in H29; eauto.
     eapply regz_exe_delay_stable2 in H29; eauto.
-    rewrite H6 in H29.
+    rewrite H9 in H29.
     inversion H29; subst.
     tryfalse.
     intro; tryfalse.
     intro; tryfalse.
     inversion H5; subst.
     inversion H27; get_ins_diff_false.
-    clear - H11.
+    eapply IHI; eauto.
+    clear - H8.
     rewrite Int.add_assoc; eauto.
 Qed.
     
 (*+ Instruction Sequence Rule Sound +*)
 Theorem wf_seq_seq_rule :
   forall p p' i q f Spec I,
-    ins_sound (p ↓) p' i -> insSeq_sound Spec p' I q ->
-    insSeq_sound Spec p (f#i;;I) q.
+    ins_sound (p ↓) p' i -> insSeq_sound Spec p' (f +ᵢ ($ 4)) I q ->
+    insSeq_sound Spec p f (i;;I) q.
 Proof.
   intros.
   unfolds insSeq_sound.
@@ -1117,14 +996,14 @@ Proof.
   {    
     eapply exe_delay_no_abort; eauto.
   }
-  simpljoin1.
+  simpljoin1. 
   renames x to R', x0 to D'.
   lets Hexe_delay : H3.
-  symmetry in H3.
+  symmetry in H3. 
   eapply dly_reduce_asrt_stable in H3; eauto.
   eapply H in H3; eauto.
   simpljoin1.
-  exists x npc (npc +ᵢ ($ 4)).
+  exists x (f +ᵢ ($ 4)) ((f +ᵢ ($ 4)) +ᵢ ($ 4)).
   destruct_state x.
   econstructor; eauto.
   eapply NTrans; eauto.
@@ -1132,8 +1011,8 @@ Proof.
   (** preservation *)
   intros.
   inversion H3; subst.
-  eapply dly_reduce_asrt_stable in H7; eauto.
-  eapply H in H7; eauto.
+  eapply dly_reduce_asrt_stable in H9; eauto.
+  eapply H in H9; eauto.
   simpljoin1.
   inversion H14; get_ins_diff_false.
   eapply ins_exec_deterministic in H4; eauto.
@@ -1142,18 +1021,18 @@ Proof.
 Qed.
 
 Theorem wf_seq_call_rule :
-  forall p q fp fq L f p1 p2 p' v i Spec r I f1 f2,
-    Spec (f, f +ᵢ ($ 4)) = Some (fp, fq) ->
-    (p ↓) ==> r15 |=> v ** p1 -> ins_sound (r15 |=> f1 ** p1 ↓) p2 i ->
-    fp L ==> Or r15 ==ₑ f1 -> p2 ==> fp L ** r ->
-    fq L ** r ==> p' -> fq L ==> Or r15 ==ₑ f1 -> DlyFrameFree r ->
-    insSeq_sound Spec p' I q ->
-    insSeq_sound Spec p (f1 c> call f;; f2 c> i;;I) q.
-Proof.
+  forall p q fp fq L f p1 p2 p' v i Spec r I f',
+    Spec f' = Some (fp, fq) ->
+    (p ↓) ==> r15 |=> v ** p1 -> ins_sound ((r15 |=> f ** p1) ↓) p2 i ->
+    p2 ==> fp L ** r ->
+    fq L ** r ==> p' -> fq L ==> Or r15 ==ₑ f -> DlyFrameFree r ->
+    insSeq_sound Spec p' (f +ᵢ ($ 8)) I q ->
+    insSeq_sound Spec p f (call f' # i # I) q.
+Proof. 
   intros.
   unfold insSeq_sound.
   intros.
-  inversion H8; subst.
+  inversion H7; subst.
   eapply call_seq; eauto.
 
   (** progress *)
@@ -1164,24 +1043,24 @@ Proof.
   }
   simpljoin1.
   renames x to R', x0 to D'.
-  lets Hexe_delay : H10.
+  lets Hexe_delay : H9.
   symmetry in Hexe_delay.
   eapply dly_reduce_asrt_stable in Hexe_delay; eauto.
   eapply H0 in Hexe_delay.
   lets Hf : Hexe_delay.
-  eapply reg_vl_change with (v1 := f1) in Hf; eauto.
-  assert (exists R'' D'', exe_delay (set_R R' r15 f1) D' = (R'', D'')).
+  eapply reg_vl_change with (v1 := f) in Hf; eauto.
+  assert (exists R'' D'', exe_delay (set_R R' r15 f) D' = (R'', D'')).
   {    
     eapply exe_delay_no_abort; eauto.
-  }
+  } 
   simpljoin1.
-  lets Hexe_delay2 : H11.
+  lets Hexe_delay2 : H10.
   renames x to R'', x0 to D''.
-  symmetry in H11.
-  eapply dly_reduce_asrt_stable in H11; eauto.
-  eapply H1 in H11; eauto.
+  symmetry in H10.
+  eapply dly_reduce_asrt_stable in H10; eauto.
+  eapply H1 in H10; eauto.
   simpljoin1.
-  exists (m, (set_R R' r15 f1, f0), D') x (f1 +ᵢ ($ 4)) f f (f +ᵢ ($ 4)).
+  exists (m, (set_R R' r15 f, f0), D') x (f +ᵢ ($ 4)) f' f' (f' +ᵢ ($ 4)).
   split; eauto.
   econstructor; eauto.
   eapply Call; eauto.
@@ -1200,45 +1079,35 @@ Proof.
 
   (** preservation *)
   intros.
-  inversion H10; subst.
-  inversion H23; get_ins_diff_false.
-  clear H18.
-  inversion H11; subst. 
-  inversion H28; get_ins_diff_false.
+  inversion H9; subst.
+  inversion H22; get_ins_diff_false.
+  clear H19.
+  inversion H10; subst. 
+  inversion H27; get_ins_diff_false.
   exists fp fq L r.
   repeat (split; eauto).
-  eapply dly_reduce_asrt_stable in H15; eauto.
-  eapply H0 in H15.
-  eapply reg_vl_change with (v1 := f1) in H15; eauto.
-  eapply dly_reduce_asrt_stable in H16; eauto.
-  eapply H1 in H16.
+  eapply dly_reduce_asrt_stable in H17; eauto.
+  eapply H0 in H17.
+  eapply reg_vl_change with (v1 := f) in H17; eauto.
+  eapply dly_reduce_asrt_stable in H17; eauto.
+  eapply H1 in H17.
   simpljoin1.
-  eapply ins_exec_deterministic in H26; eauto.
+  eapply ins_exec_deterministic in H25; eauto.
   simpljoin1.
   eauto.
   intros.
-  eapply H4 in H12.
-  clear - H7 H21 H12.
+  eapply H3 in H11.
+  clear - H6 H16 H11.
   unfolds insSeq_sound.
-  eapply H7 in H21; eauto.
-  do 2 rewrite Int.add_assoc in H21; eauto.
-  eapply H2 in H12.
-  clear - H12.
-  destruct_state S'.
-  simpls.
-  eauto.
-  eapply H5 in H13.
-  clear - H13.
-  destruct_state S''.
-  simpls.
-  eauto.
+  eapply H6 in H16; eauto.
+  rewrite Int.add_assoc in H16; eauto.
 Qed.
 
 Theorem wf_seq_ret_rule :
-  forall p p' q i Spec f1 f2,
+  forall p p' q i Spec f,
     ins_sound ((p ↓) ↓) p' i ->
     p' ==> q -> fretSta ((p ↓) ↓) p' ->
-    insSeq_sound Spec p (f1 r> retl ;; f2 r> i) q.
+    insSeq_sound Spec p f (retl ;; i) q.
 Proof.
   intros.
   unfolds insSeq_sound.
@@ -1260,27 +1129,27 @@ Proof.
   assert (exists R'' D'', exe_delay R' D' = (R'', D'')).
   {
     eapply exe_delay_no_abort; eauto.
-  }
+  } 
   simpljoin1.
   renames x to R'', x0 to D''.
-  symmetry in H5.
-  lets Hexe_delay2 : H5. 
+  symmetry in H6.
+  lets Hexe_delay2 : H6. 
   eapply dly_reduce_asrt_stable in Hexe_delay2; eauto.
   lets Hp' : Hexe_delay2.
   eapply H in Hp'; eauto.
   simpljoin1.
-  lets Hret_f : H7.
+  lets Hret_f : H9.
   eapply H1 in Hret_f; eauto.
   simpljoin1. 
-  exists (m, (R', f), D') x f2 (x0 +ᵢ ($ 8)) (x0 +ᵢ ($ 8)) ((x0 +ᵢ ($ 8)) +ᵢ ($ 4)).
-  split; eauto.
+  exists (m, (R', f0), D') x (f +ᵢ ($ 4)) (x0 +ᵢ ($ 8)) (x0 +ᵢ ($ 8)) ((x0 +ᵢ ($ 8)) +ᵢ ($ 4)).
+  split; eauto. 
   econstructor; eauto.
   eapply Retl; eauto.
   simpls. 
-  clear - H5 H8.
+  clear - H6 H10.
   unfolds get_R.
-  eapply exe_delay_general_reg_stable in H8; eauto.
-  rewrite H8; eauto.
+  eapply exe_delay_general_reg_stable in H10; eauto.
+  rewrite H10; eauto.
   destruct_state x.
   econstructor; eauto.
   eapply NTrans; eauto.
@@ -1290,11 +1159,11 @@ Proof.
   inversion H4; subst.
   inversion H16; get_ins_diff_false.
   clear H12.
-  inversion H5; subst.
+  inversion H6; subst.
   inversion H21; get_ins_diff_false.
-  lets Hexe_delay1 : H10.
+  lets Hexe_delay1 : H11.
   lets Hexe_delay2 : H12.
-  eapply dly_reduce_asrt_stable in H10; eauto.
+  eapply dly_reduce_asrt_stable in H11; eauto.
   eapply dly_reduce_asrt_stable in H12; eauto.
   lets Hp' : H12.
   eapply H in Hp'; eauto.
@@ -1302,10 +1171,10 @@ Proof.
   eapply ins_exec_deterministic in H19; eauto.
   subst.
   split; eauto.
-  exists f.
+  exists f0.
   simpl.
   repeat (split; eauto).
-  eapply H1 in H7; eauto.
+  eapply H1 in H9; eauto.
   simpljoin1.
   simpls.
   symmetry in Hexe_delay2.
@@ -1315,19 +1184,19 @@ Proof.
   2 : intro; tryfalse.
   eapply exe_delay_general_reg_stable with (r := r15) in Hexe_delay2; eauto.
   eapply Hexe_delay2 in H24.
-  rewrite H24 in H7.
-  inversion H7; subst.
+  rewrite H24 in H9.
+  inversion H9; subst.
   eauto.
   rewrite Int.add_assoc; eauto.
 Qed.
 
 Theorem wf_seq_j1_rule :
-  forall f1 f2 f aexp (r1 : GenReg) i p p' p1 q fp fq r Spec L v,
-    Spec (f, f +ᵢ ($ 4)) = Some (fp, fq) ->
-    (p ↓) ==> aexp ==ₓ f -> (p ↓) ==> r1 |=> v ** p1 ->
-    ins_sound (r1 |=> f1 ** p1 ↓) p' i ->
+  forall f f' aexp (r1 : GenReg) i p p' p1 q fp fq r Spec L v,
+    Spec f' = Some (fp, fq) ->
+    (p ↓) ==> aexp ==ₓ f' -> (p ↓) ==> r1 |=> v ** p1 ->
+    ins_sound ((r1 |=> f ** p1) ↓) p' i ->
     p' ==> fp L ** r -> fq L ** r ==> q -> DlyFrameFree r ->
-    insSeq_sound Spec p (consJ1 f1 aexp r1 f2 i) q.
+    insSeq_sound Spec p f (consJ aexp r1 i) q.
 Proof.
   intros.
   unfold insSeq_sound.
@@ -1351,8 +1220,8 @@ Proof.
   eapply H0 in Haexp.
   eapply H1 in Hf1.
   lets Hf1' : Hf1.
-  eapply reg_vl_change with (v1 := f1) in Hf1'; eauto.
-  assert (exists R'' D'', exe_delay (set_R R' r1 f1) D' = (R'', D'')).
+  eapply reg_vl_change with (v1 := f) in Hf1'; eauto.
+  assert (exists R'' D'', exe_delay (set_R R' r1 f) D' = (R'', D'')).
   {
     eapply exe_delay_no_abort; eauto.
   }
@@ -1363,7 +1232,7 @@ Proof.
   eapply dly_reduce_asrt_stable in Hexe_delay2; eauto.
   eapply H2 in Hexe_delay2; eauto.
   simpljoin1. 
-  exists (m, (set_R R' r1 f1, f0), D') x f2 f f (f +ᵢ ($ 4)).
+  exists (m, (set_R R' r1 f, f0), D') x (f +ᵢ ($ 4)) f' f' (f' +ᵢ ($ 4)).
   split; eauto.
   econstructor; eauto.
   eapply Jumpl; eauto.
@@ -1389,9 +1258,9 @@ Proof.
   (** preservation *)
   intros.
   inversion H8; subst.
-  eapply dly_reduce_asrt_stable in H14; eauto.
-  lets Haexp : H14.
-  lets Hf1 : H14.
+  eapply dly_reduce_asrt_stable in H15; eauto.
+  lets Haexp : H15.
+  lets Hf1 : H15.
   eapply H0 in Haexp.
   simpl in Haexp.
   simpljoin1.
@@ -1404,7 +1273,7 @@ Proof.
   exists fp fq L r.
   repeat (split; eauto).
   eapply H1 in Hf1.
-  eapply reg_vl_change with (v1 := f1) in Hf1; eauto.
+  eapply reg_vl_change with (v1 := f) in Hf1; eauto.
   eapply dly_reduce_asrt_stable in H18; eauto.
   eapply H2 in H18; eauto.
   simpljoin1.
@@ -1413,116 +1282,14 @@ Proof.
   eauto.
 Qed.
 
-Theorem wf_seq_J2_rule :
-  forall p p1 p2 q f1 f1' f2 f2' aexp1 aexp2 (r1 r2 : GenReg) fp fq L r Spec v1 v2,
-    Spec (f1', f2') = Some (fp, fq) ->
-    (p ↓) ==> aexp1 ==ₓ f1' -> (p ↓) ==> r1 |=> v1 ** p1 ->
-    (r1 |=> f1 ** p1 ↓) ==> aexp2 ==ₓ f2' -> (r1 |=> f1 ** p1 ↓) ==> r2 |=> v2 ** p2 ->
-    r2 |=> f2 ** p2 ==> fp L ** r -> fq L ** r ==> q -> DlyFrameFree r ->
-    insSeq_sound Spec p (consJ2 f1 aexp1 r1 f2 aexp2 r2) q.
-Proof.
-  intros.
-  unfold insSeq_sound.
-  intros.
-  inversion H7; subst.
-  eapply jmpl_seq; eauto.
-
-  (** progress *)
-  destruct_state S.
-  assert (exists R' D', exe_delay r0 d = (R', D')).
-  {
-    eapply exe_delay_no_abort; eauto.
-  }
-  simpljoin1.
-  renames x to R', x0 to D'.
-  lets Hexe_delay1 : H9.
-  symmetry in Hexe_delay1.
-  eapply dly_reduce_asrt_stable in Hexe_delay1; eauto.
-  lets Haexp1 : Hexe_delay1.
-  lets Hf1 : Hexe_delay1.
-  eapply H0 in Haexp1.
-  eapply H1 in Hf1.
-  lets Hf1' : Hf1.
-  eapply reg_vl_change with (v1 := f1) in Hf1; eauto.
-  assert (exists R'' D'', exe_delay (set_R R' r1 f1) D' = (R'', D'')).
-  {
-    eapply exe_delay_no_abort; eauto.
-  }
-  simpljoin1.
-  renames x to R'', x0 to D''.
-  lets Hexe_delay2 : H10.
-  symmetry in Hexe_delay2.
-  eapply dly_reduce_asrt_stable in Hexe_delay2; eauto.
-  lets Haexp2 : Hexe_delay2.
-  lets Hf2 : Hexe_delay2.
-  eapply H2 in Haexp2; eauto.
-  eapply H3 in Hf2; eauto.
-  simpl in Haexp1.
-  simpl in Haexp2.
-  simpljoin1.
-  exists (m, (set_R R' r1 f1, f), D') (m, (set_R R'' r2 f2, f), D'') f2 f1' f1' f2'.
-  split; eauto.
-  econstructor; eauto.
-  eapply Jumpl; eauto.
-  clear - Hf1'.
-  sep_star_split_tac.
-  simpls.
-  unfolds regSt.
-  simpls.
-  simpljoin1.
-  eapply indom_merge_still; eauto.
-  eapply regset_l_l_indom; eauto.
-  econstructor; eauto.
-  eapply Jumpl; eauto.
-  clear - Hf2.
-  sep_star_split_tac.
-  simpls.
-  unfolds regSt.
-  simpls.
-  simpljoin1.
-  eapply indom_merge_still; eauto.
-  eapply regset_l_l_indom; eauto.
-
-  (** preservation *)
-  intros.
-  inversion H9; subst.
-  eapply dly_reduce_asrt_stable in H15; eauto.
-  lets Haexp1 : H15.
-  lets Hf1 : H15.
-  eapply H0 in Haexp1.
-  eapply H1 in Hf1.
-  inversion H21; get_ins_diff_false.
-  simpl in Haexp1.
-  simpljoin1.
-  rewrite H11 in H29.
-  inversion H29; subst.
-  clear H29.
-  inversion H10; subst.
-  lets Hf1' : Hf1.
-  eapply reg_vl_change with (v1 := f1) in Hf1'; eauto.
-  eapply dly_reduce_asrt_stable in H18; eauto.
-  lets Haexp2 : H18.
-  lets Hf2 : H18.
-  eapply H2 in Haexp2.
-  eapply H3 in Hf2.
-  simpl in Haexp2.
-  simpljoin1.
-  inversion H28; get_ins_diff_false.
-  rewrite H13 in H37.
-  inversion H37; subst.
-  exists fp fq L r.
-  repeat (split; eauto).
-  eapply reg_vl_change with (v1 := pc1) in Hf2; eauto.
-Qed.
-
 Lemma wf_seq_be_rule :
-  forall p p' q r f1 f2 f i fp fq L I bv Spec,
-    Spec (f, f +ᵢ ($ 4)) = Some (fp, fq) -> DlyFrameFree r ->
-    (p ↓) ==> z |=> bv ** Atrue ->
+  forall p p' q r f f' i fp fq L I bv Spec,
+    Spec f' = Some (fp, fq) -> DlyFrameFree r ->
+    p ==> z |=> bv ** Atrue ->
     ins_sound ((p ↓) ↓) p' i ->
     (bv =ᵢ ($ 0) = false -> p' ==> fp L ** r /\ fq L ** r ==> q) ->
-    (bv =ᵢ ($ 0) = true -> insSeq_sound Spec p' I q) ->
-    insSeq_sound Spec p (f1 e> be f;; f2 e> i;;I) q.
+    (bv =ᵢ ($ 0) = true -> insSeq_sound Spec p' (f +ᵢ ($ 8)) I q) ->
+    insSeq_sound Spec p f (be f'# i#I) q.
 Proof. 
   introv H Hr.
   intros.
@@ -1553,15 +1320,18 @@ Proof.
   eapply dly_reduce_asrt_stable in Hp'; eauto.
   eapply H1 in Hp'.
   simpljoin1.
-  lets Hz : Hp.
+  lets Hz : H5.
   eapply H0 in Hz.
   destruct (Int.eq bv ($ 0)) eqn:Heqe.
   {
-    exists (m, (R', f0), D') x f2 (f2 +ᵢ ($ 4)) (f2 +ᵢ ($ 4)) ((f2 +ᵢ ($ 4)) +ᵢ ($ 4)).
+    exists (m, (R', f0), D') x (f +ᵢ ($ 4)) ((f +ᵢ ($ 4)) +ᵢ ($ 4))
+      ((f +ᵢ ($ 4)) +ᵢ ($ 4)) (((f +ᵢ ($ 4)) +ᵢ ($ 4)) +ᵢ ($ 4)).
     split; eauto.
     econstructor; eauto.
-    eapply Be_false with (f := f); eauto.
-    clear - Heqe Hz.
+    eapply Be_false with (f := f'); eauto.
+    clear - Heqe Hz H6.
+    rewrite get_R_rn_neq_r0; eauto.
+    eapply regz_exe_delay_stable; eauto.    
     sep_star_split_tac.
     simpls.
     simpljoin1.
@@ -1569,33 +1339,32 @@ Proof.
     simpls.
     simpljoin1. 
     eapply int_eq_true_eq in Heqe.
-    rewrite get_R_rn_neq_r0; eauto.
-    unfold merge.
+    eapply get_vl_merge_still; eauto.
     subst.
     unfold RegMap.set.
-    destruct_rneq; eauto.
+    destruct_rneq.
     intro; tryfalse.
     destruct_state x.
     econstructor; eauto.
     eapply NTrans; eauto.
   }
   {  
-    exists (m, (R', f0), D') x f2 f f (f +ᵢ ($ 4)).
+    exists (m, (R', f0), D') x (f +ᵢ ($ 4)) f' f' (f' +ᵢ ($ 4)).
     split; eauto.
     econstructor; eauto.
     eapply Be_true with (v := bv); eauto.
-    clear - Hz.
+    clear - Hz H6.
+    rewrite get_R_rn_neq_r0; eauto. 
+    eapply regz_exe_delay_stable; eauto.
     sep_star_split_tac.
     simpls.
     unfolds regSt.
     simpls.
     simpljoin1.
-    rewrite get_R_rn_neq_r0; eauto.
-    2 : intro; tryfalse.
-    unfold merge.
+    eapply get_vl_merge_still; eauto.
     unfold RegMap.set.
     destruct_rneq.
-    clear - Heqe.
+    intro; tryfalse.
     eapply int_eq_false_neq in Heqe; eauto.
     destruct_state x.
     econstructor; eauto.
@@ -1608,13 +1377,14 @@ Proof.
   inversion H7; subst.
   exists bv.
   split; eauto.
-  lets Hexe_delay1 : H11.
-  eapply dly_reduce_asrt_stable in H11; eauto.
+  lets Hexe_delay1 : H14.
+  eapply dly_reduce_asrt_stable in H14; eauto.
   inversion H19; get_ins_diff_false.
-  eapply dly_reduce_asrt_stable in H13; eauto.
-  clear H17. 
-  eapply H0 in H11.  
-  clear - Hexe_delay1 H11 H29.
+  eapply dly_reduce_asrt_stable in H15; eauto.
+  clear H17.
+  lets Hz : H5.
+  eapply H0 in Hz.  
+  clear - Hz.
   sep_star_split_tac.
   simpls. 
   unfolds regSt.
@@ -1622,8 +1392,9 @@ Proof.
   simpljoin1.
   rewrite get_R_rn_neq_r0; eauto.
   2 : intro; tryfalse.
-  rewrite get_R_rn_neq_r0 in H29; eauto.
-  2 : intro; tryfalse.
+  eapply get_vl_merge_still; eauto.
+  unfold RegMap.set.
+  destruct_rneq.
   lets Hz : H29.
   unfold merge in Hz.
   unfold RegMap.set in Hz.
